IR staffs

examples/dev/sw/IL.sml
@@ -180,36 +180,60 @@ val translate = Define `
   `;
 
 (*---------------------------------------------------------------------------------*)
-(*      Operational Semantics of programs in intermedia language                   *)
+(*      Intermediate Representation                                                *)
+(*      Definition of run_ir                                                       *) 
 (*---------------------------------------------------------------------------------*)
+
+val run_arm = Define `
+      run_arm arm ((pc,cpsr,st),pcS) = runTo (upload arm (\i.ARB) pc) (pc+LENGTH arm) ((pc,cpsr,st),pcS)`;
 
 val run_ir = Define `
-     (run_ir (BLK (stm::stmL)) st =
-          run_ir (BLK stmL) (mdecode st stm)) /\
-     (run_ir (BLK []) st =
-          st) /\
-
-     (run_ir (SC S1 S2) st = 
-          run_ir S2 (run_ir S1 st)) /\
-
-     (run_ir (CJ cond Strue Sfalse) st = 
-          if eval_cond cond st then 
-              run_ir Strue st
-          else
-              run_ir Sfalse st) /\
-
-     (run_ir (TR cond Sbody) st =
-         WHILE (\s.eval_cond cond s) (run_ir Sbody) st)
-    `;
+      run_ir ir st = get_st (run_arm (translate ir) ((0,0w,st),{}))`;
 
 (*---------------------------------------------------------------------------------*)
-(*      Stack Behaviors                                                            *)
+(*      Hoare Rules for IR                                                         *) 
 (*---------------------------------------------------------------------------------*)
 
+val HOARE_SC_IR = Q.store_thm (
+   "HOARE_SC_IR",
+   `!ir1 ir2 P Q R T.
+       well_formed (translate ir1) /\ well_formed (translate ir2) /\
+           (!st. P st ==> Q (run_ir ir1 st)) /\
+           (!st. R st ==> T (run_ir ir2 st)) /\ (!st. Q st ==> R st) ==>
+             !st. P st ==>
+                  T (run_ir (SC ir1 ir2) st)`,
+   RW_TAC std_ss [run_ir, translate, run_arm, eval_fl] THEN 
+   IMP_RES_TAC (SIMP_RULE std_ss [eval_fl, uploadCode_def]  HOARE_SC_FLAT)
+  );
 
-(*--------------------------------------------------------------------------------------------*)
-(*      Sanity and Correctness of the translation from intermediate language to flat code     *)
-(*--------------------------------------------------------------------------------------------*)
+val HOARE_CJ_IR = Q.store_thm (
+   "HOARE_CJ_IR",
+   `!cond ir_t ir_f P Q R.
+       well_formed (translate ir_t) /\ well_formed (translate ir_f) /\
+           (!st. P st ==> Q (run_ir ir_t st)) /\
+           (!st. P st ==> R (run_ir ir_f st)) ==>
+             !st. P st ==>
+                if eval_cond cond st then Q (run_ir (CJ cond ir_t ir_f) st)
+                    else R (run_ir (CJ cond ir_t ir_f) st)`,
+   RW_TAC std_ss [run_ir, translate, run_arm, eval_fl] THEN
+   IMP_RES_TAC (SIMP_RULE std_ss [eval_fl, uploadCode_def] HOARE_CJ_FLAT) THEN
+   METIS_TAC []
+  );
+
+val HOARE_TR_IR = Q.store_thm (
+   "HOARE_TR_IR",
+   `!cond ir P.
+       well_formed (translate ir) /\  WF_TR (cond, translate ir) /\
+         (!st. P st ==> P (run_ir ir st)) ==>
+            !st. P st ==> P (run_ir (TR cond ir) st) /\ 
+                 eval_cond cond (run_ir (TR cond ir) st)`,
+   RW_TAC std_ss [run_ir, translate, run_arm, eval_fl] THEN
+   METIS_TAC [SIMP_RULE std_ss [eval_fl, uploadCode_def] HOARE_TR_FLAT]
+  );
+
+(*---------------------------------------------------------------------------------*)
+(*      Well-formedness of IR                                                      *) 
+(*---------------------------------------------------------------------------------*)
 
 val UPLOAD_LEM_2 = Q.store_thm (
    "UPLOAD_LEM_2",
@@ -250,7 +274,6 @@ val STATEMENT_IS_WELL_FORMED = Q.store_thm (
 val BLOCK_IS_WELL_FORMED = Q.store_thm (
    "BLOCK_IS_WELL_FORMED",
    `!stmL. well_formed (translate (BLK stmL))`,
-
     Induct_on `stmL` THENL [
         RW_TAC list_ss [well_formed, translate, closed, terminated, status_independent, stopAt_def] THENL [
             RW_TAC set_ss [Once RUNTO_ADVANCE],
@@ -262,3 +285,207 @@ val BLOCK_IS_WELL_FORMED = Q.store_thm (
     ]
 );
 
+val IR_SC_IS_WELL_FORMED = Q.store_thm (
+   "IR_SC_IS_WELL_FORMED",
+   `!ir1 ir2. well_formed (translate ir1) /\ well_formed (translate ir2) ==>
+        well_formed (translate (SC ir1 ir2))`,
+    RW_TAC std_ss [translate] THEN
+    IMP_RES_TAC (SC_IS_WELL_FORMED)
+   );
+
+val IR_CJ_IS_WELL_FORMED = Q.store_thm (
+   "IR_CJ_IS_WELL_FORMED",
+   `!cond ir_t ir_f. well_formed (translate ir_t) /\ well_formed (translate ir_f) ==>
+        well_formed (translate (CJ cond ir_t ir_f))`,
+    RW_TAC std_ss [translate] THEN
+    IMP_RES_TAC (CJ_IS_WELL_FORMED) THEN
+    METIS_TAC []
+   );
+
+val IR_TR_IS_WELL_FORMED = Q.store_thm (
+   "IR_TR_IS_WELL_FORMED",
+   `!ir cond. well_formed (translate ir) /\ WF_TR (cond, translate ir) ==>
+        well_formed (translate (TR cond ir))`,
+    RW_TAC std_ss [translate] THEN
+    IMP_RES_TAC (TR_IS_WELL_FORMED)
+   );
+
+(*---------------------------------------------------------------------------------*)
+(*      Semantics of IR                                                            *) 
+(*---------------------------------------------------------------------------------*)
+
+val IR_SEMANTICS_SC = Q.store_thm (
+   "IR_SEMANTICS_SC",
+   `well_formed (translate ir1) /\ well_formed (translate ir2) ==>
+     (run_ir (SC ir1 ir2) st =
+       run_ir ir2 (run_ir ir1 st))`,
+    METIS_TAC [SIMP_RULE std_ss [] (Q.SPECL [`ir1`,`ir2`, `\st'. st' = st`, `\st'. st' = run_ir ir1 st`, `\st'. st' = run_ir ir1 st`,
+                         `\st'. st' =  run_ir ir2 (run_ir ir1 st)`] HOARE_SC_IR)]
+   );
+   
+ 
+val IR_SEMANTICS_BLK = Q.store_thm (
+   "IR_SEMANTICS_BLK",
+    `(run_ir (BLK (stm::stmL)) st =
+          run_ir (BLK stmL) (mdecode st stm)) /\
+     (run_ir (BLK []) st = st)`,
+
+    REPEAT STRIP_TAC THENL [
+       RW_TAC list_ss [run_ir, translate] THEN
+           `translate_assignment stm::translate (BLK stmL) = translate (SC (BLK [stm]) (BLK stmL))` by RW_TAC list_ss [translate,mk_SC] THEN
+           RW_TAC std_ss [GSYM run_ir] THEN
+           `run_ir (BLK [stm]) st = mdecode st stm` by (
+               RW_TAC list_ss [run_ir, run_arm, translate, Once RUNTO_ADVANCE] THEN
+               RW_TAC list_ss [GSYM uploadCode_def, UPLOADCODE_LEM] THEN
+               RW_TAC list_ss [GSYM TRANSLATE_ASSIGMENT_CORRECT, get_st, Once RUNTO_ADVANCE]
+           ) THEN
+           `well_formed [translate_assignment stm] /\ well_formed (translate (BLK stmL))` by 
+               METIS_TAC [BLOCK_IS_WELL_FORMED, STATEMENT_IS_WELL_FORMED] THEN
+           FULL_SIMP_TAC list_ss [IR_SEMANTICS_SC, translate],
+       RW_TAC list_ss [run_ir, run_arm, translate, Once RUNTO_ADVANCE, get_st]
+   ]
+  );
+
+val IR_SEMANTICS_CJ = Q.store_thm (
+   "IR_SEMANTICS_CJ",
+   ` well_formed (translate ir_t) /\ well_formed (translate ir_f) ==>
+     (run_ir (CJ cond ir_t ir_f) st = 
+          if eval_cond cond st then run_ir ir_t st
+          else run_ir ir_f st)`,
+   RW_TAC std_ss [] THEN
+   METIS_TAC [SIMP_RULE std_ss [] (Q.SPECL [`cond`, `ir_t`, `ir_f`, `\st'. st' = st`, `\st'. st' = run_ir ir_t st`, 
+                 `\st'. st' = run_ir ir_f st`] HOARE_CJ_IR)]
+  );
+
+
+val IR_SEMANTICS_TR = Q.store_thm (
+   "IR_SEMANTICS_TR",
+     `well_formed (translate ir) /\ WF_TR (cond,translate ir) ==>
+      (run_ir (TR cond ir) st =
+         WHILE (\st'.~eval_cond cond st') (run_ir ir) st)`,
+
+    RW_TAC std_ss [run_ir, run_arm, translate] THEN
+    Q.ABBREV_TAC `arm = translate ir` THEN
+    IMP_RES_TAC (SIMP_RULE set_ss [] (Q.SPECL [`cond`,`arm`,`(\i. ARB)`,`(0,0w,st):STATE`,`{}`] UNROLL_TR_LEM)) THEN
+    POP_ASSUM (ASSUME_TAC o Q.SPEC `st`) THEN
+    FULL_SIMP_TAC std_ss [FUNPOW,get_st] THEN
+    NTAC 2 (POP_ASSUM (K ALL_TAC)) THEN
+    Induct_on `loopNum cond arm (\i.ARB) ((0,0w,st),{})` THENL [
+        REWRITE_TAC [Once EQ_SYM_EQ] THEN RW_TAC std_ss [FUNPOW,get_st] THEN
+            IMP_RES_TAC LOOPNUM_BASIC THEN
+            FULL_SIMP_TAC arith_ss [Once WHILE, get_st],
+
+        REWRITE_TAC [Once EQ_SYM_EQ] THEN RW_TAC std_ss [FUNPOW] THEN
+            IMP_RES_TAC LOOPNUM_INDUCTIVE THEN
+            `v = loopNum cond arm (\i.ARB) ((0,0w,SND (SND (FST (runTo (upload arm (\i.ARB) 0) (LENGTH arm) ((0,0w,st),{}))))),{})` by
+            METIS_TAC [ABS_PAIR_THM,DECIDE (Term`!x.0+x=x`),LOOPNUM_INDEPENDENT_OF_CPSR_PCS, get_st, FST, SND, DSTATE_IRRELEVANT_PCS, well_formed] THEN
+            RES_TAC THEN Q.PAT_ASSUM `v = x` (ASSUME_TAC o GSYM) THEN FULL_SIMP_TAC std_ss [] THEN POP_ASSUM (K ALL_TAC) THEN
+            Q.PAT_ASSUM `v = x` (ASSUME_TAC o GSYM) THEN FULL_SIMP_TAC std_ss [] THEN POP_ASSUM (K ALL_TAC) THEN
+            Q.PAT_ASSUM `~x` (ASSUME_TAC o SIMP_RULE std_ss [get_st]) THEN
+            RW_TAC std_ss [Once WHILE] THEN
+            Q.UNABBREV_TAC `arm` THEN
+            `run_ir ir st = SND (SND (FST (runTo (upload (translate ir) (\i. ARB) 0) (LENGTH (translate ir)) ((0,0w,st),{}))))` by RW_TAC arith_ss [
+                   get_st, run_ir, run_arm] THEN 
+            METIS_TAC [SND,FST,get_st,FUNPOW_DSTATE, ABS_PAIR_THM]
+      ]
+  );
+
+
+val SEMANTICS_OF_IR = Q.store_thm (
+   "SEMANTICS_OF_IR",
+   ` well_formed (translate ir1) /\ well_formed (translate ir2) ==>
+     (run_ir (BLK (stm::stmL)) st =
+          run_ir (BLK stmL) (mdecode st stm)) /\
+     (run_ir (BLK []) st = st) /\
+     (run_ir (SC ir1 ir2) st = run_ir ir2 (run_ir ir1 st)) /\
+     (run_ir (CJ cond ir1 ir2) st =
+           (if eval_cond cond st then run_ir ir1 st else run_ir ir2 st)) /\
+     ( WF_TR (cond,translate ir1) ==> 
+       (run_ir (TR cond ir1) st =
+           WHILE (\st'. ~eval_cond cond st') (run_ir ir1) st))`,
+   RW_TAC std_ss [IR_SEMANTICS_BLK, IR_SEMANTICS_CJ, IR_SEMANTICS_SC, IR_SEMANTICS_TR]
+  );       
+
+(*---------------------------------------------------------------------------------*)
+(*      Hoare Rules on Projection on Inputs and Ouputs                             *) 
+(*---------------------------------------------------------------------------------*)
+
+val prj_f = Define `
+      prj_f st expL = MAP (read st) expL`;
+
+val HOARE_SC_PROJECTION = Q.store_thm (
+   "HOARE_SC_PROJECTION",
+   `!ir1 ir2 f1 f2 ins1 outs1 outs2 . 
+     well_formed (translate ir1) /\ well_formed (translate ir2) /\
+     (!v st. (prj_f st ins1 = v) ==> (prj_f (run_ir ir1 st) outs1 = f1 v)) /\
+     (!v st. (prj_f st outs1 = v) ==> (prj_f (run_ir ir2 st) outs2 = f2 v)) 
+       ==>
+     (!v st. (prj_f st ins1 = v) ==> (prj_f (run_ir (SC ir1 ir2) st) outs2 = (f2 o f1) v))`,
+
+     REPEAT STRIP_TAC THEN
+     IMP_RES_TAC (SIMP_RULE std_ss [] (Q.SPECL [`ir1`,`ir2`, `\st. prj_f st ins1 = v`, `\st.prj_f st outs1 = (f1:DATA list->DATA list) v`, 
+          `\st'. prj_f st' outs1 = (f1:DATA list->DATA list) v`, `\st. prj_f st outs2 = ((f2:DATA list->DATA list) o (f1:DATA list->DATA list)) v`] 
+              HOARE_SC_IR)) THEN
+     NTAC 13 (POP_ASSUM (K ALL_TAC)) THEN
+     POP_ASSUM (MP_TAC o Q.SPECL [`v`,`outs1`,`ins1`,`f1:DATA list->DATA list`]) THEN
+     NTAC 2 (POP_ASSUM (K ALL_TAC)) THEN STRIP_TAC THEN
+     FULL_SIMP_TAC list_ss []
+   );
+
+val HOARE_CJ_PROJECTION = Q.store_thm (
+   "HOARE_CJ_PROJECTION",
+   `!ir1 ir2 f1 f2 ins outs . 
+     well_formed (translate ir_t) /\ well_formed (translate ir_f) /\
+     (!v st. (prj_f st ins = v) ==> (prj_f (run_ir ir_t st) outs = f1 v)) /\
+     (!v st. (prj_f st ins = v) ==> (prj_f (run_ir ir_f st) outs = f2 v)) 
+       ==>
+     !v st. (prj_f st ins = v) ==> 
+        (prj_f (run_ir (CJ cond ir_t ir_f) st) outs = if eval_cond cond st then f1 v 
+                                      else f2 v)`,
+
+     REPEAT STRIP_TAC THEN
+     IMP_RES_TAC (SIMP_RULE std_ss [] (Q.SPECL [`cond`,`ir_t`,`ir_f`, `\st. prj_f st ins = v`, `\st.prj_f st outs = (f1:DATA list->DATA list) v`, 
+          `\st. prj_f st outs = (f2:DATA list->DATA list) v`] HOARE_CJ_IR)) THEN
+     NTAC 13 (POP_ASSUM (K ALL_TAC)) THEN
+     POP_ASSUM (MP_TAC o Q.SPECL [`v`,`outs`,`ins`,`f1:DATA list->DATA list`]) THEN
+     NTAC 2 (POP_ASSUM (K ALL_TAC)) THEN STRIP_TAC THEN
+     REPEAT (Q.PAT_ASSUM `!v st.x` (ASSUME_TAC o Q.SPEC `v`)) THEN RES_TAC THEN
+     RW_TAC std_ss [] THEN METIS_TAC []
+   );
+
+(*
+val HOARE_TR_PROJECTION = Q.store_thm (
+   "HOARE_TR_PROJECTION",
+   `!ir f ins outs . 
+     well_formed (translate ir) /\
+     (!v st. (prj_f st ins = v) ==> (prj_f (run_ir ir_t st) outs = f v)) 
+       ==>
+     !v st. (prj_f st ins = v) ==> 
+        (prj_f (run_ir (TR cond ir) st) outs = WHILE (\v'. eval_cond cond v') f v)`,
+
+    RW_TAC std_ss [run_ir, run_arm, translate] THEN
+    Q.ABBREV_TAC `arm = translate ir` THEN
+    IMP_RES_TAC (SIMP_RULE set_ss [] (Q.SPECL [`cond`,`arm`,`(\i. ARB)`,`(0,0w,st):STATE`,`{}`] UNROLL_TR_LEM)) THEN
+    POP_ASSUM (ASSUME_TAC o Q.SPEC `st`) THEN
+    FULL_SIMP_TAC std_ss [FUNPOW,get_st] THEN
+    NTAC 2 (POP_ASSUM (K ALL_TAC)) THEN
+    Induct_on `loopNum cond arm (\i.ARB) ((0,0w,st),{})` THENL [
+        REWRITE_TAC [Once EQ_SYM_EQ] THEN RW_TAC std_ss [FUNPOW,get_st] THEN
+            IMP_RES_TAC LOOPNUM_BASIC THEN
+            FULL_SIMP_TAC arith_ss [Once WHILE, get_st],
+
+        REWRITE_TAC [Once EQ_SYM_EQ] THEN RW_TAC std_ss [FUNPOW] THEN
+            IMP_RES_TAC LOOPNUM_INDUCTIVE THEN
+            `v = loopNum cond arm (\i.ARB) ((0,0w,SND (SND (FST (runTo (upload arm (\i.ARB) 0) (LENGTH arm) ((0,0w,st),{}))))),{})` by
+            METIS_TAC [ABS_PAIR_THM,DECIDE (Term`!x.0+x=x`),LOOPNUM_INDEPENDENT_OF_CPSR_PCS, get_st, FST, SND, DSTATE_IRRELEVANT_PCS, well_formed] THEN
+            RES_TAC THEN Q.PAT_ASSUM `v = x` (ASSUME_TAC o GSYM) THEN FULL_SIMP_TAC std_ss [] THEN POP_ASSUM (K ALL_TAC) THEN
+            Q.PAT_ASSUM `v = x` (ASSUME_TAC o GSYM) THEN FULL_SIMP_TAC std_ss [] THEN POP_ASSUM (K ALL_TAC) THEN
+            Q.PAT_ASSUM `~x` (ASSUME_TAC o SIMP_RULE std_ss [get_st]) THEN
+            RW_TAC std_ss [Once WHILE] THEN
+            Q.UNABBREV_TAC `arm` THEN
+            `run_ir ir st = SND (SND (FST (runTo (upload (translate ir) (\i. ARB) 0) (LENGTH (translate ir)) ((0,0w,st),{}))))` by RW_TAC arith_ss [
+                   get_st, run_ir, run_arm] THEN 
+            METIS_TAC [SND,FST,get_st,FUNPOW_DSTATE, ABS_PAIR_THM]
+      ]
+   );
+*)
